coq-osiris/theories/program_logic/handler_rules.v
@@ -281,18 +281,6 @@ Section handler_proof.
       iModIntro. rewrite /continue.
       iApply ("IH" with "He Hsh"). }
 
-    { (* StepHandleDie] *)
-      ewp_mask_intro "Hmod". iModIntro. ewp_mask_elim. iFrame.
-      rewrite ewp_unfold /ewp_pre /=.
-      ewp_unfold_head.
-      intro_state. spec_state. iModIntro.
-      construct_wp_nonret. destruct_wp_step.
-      epose proof (DieS _ _ _ _ _ H) as Hstep0.
-      iSpecialize ("He" $! _ _ _ _ Hstep0).
-      ewp_mask_elim. iMod "He" as "($ & He & _)".
-      iModIntro. rewrite /continue.
-      iApply ("IH" with "He Hsh"). }
-
     { (* [StepHandleCrash] *)
       by ewp_invert. }
 
