coq-osiris/theories/semantics/pure_step.v
@@ -30,7 +30,6 @@ Ltac inv_ipure :=
   | h: ipure (Stop CFork _ _) |- _ => inv h
   | h: ipure (Stop CJoin _ _) |- _ => inv h
   | h: ipure (Stop CSelf _ _) |- _ => inv h
-  | h: ipure (Stop CDie _ _) |- _ => inv h
   end.
 
 Local Lemma may_pure_step {A E} (m : micro A E) :
